protocols/PartialOrderReduction.v
@@ -38,7 +38,9 @@ From protocols Require Import
      ExampleProtocols
      ModelCheck
      ProtocolAutomation
-     SafeProtocol.
+     SafeProtocol
+     SyntacticallySafe
+     RealWorldStepLemmas.
 
 From protocols Require Sets.
 
@@ -256,180 +258,6 @@ Section RealWorldLemmas.
         eapply StepBindRecur; eauto 12.
   Qed.
 
-  (* need to know that msg, if cipher, is in cs *)
-  Lemma findKeysCrypto_addnl_cipher :
-    forall {t} (msg : crypto t) cs c_id c,
-      ~ In c_id cs
-      -> (forall cid, msg_cipher_id msg = Some cid -> cs $? cid <> None)
-      -> findKeysCrypto cs msg = findKeysCrypto (cs $+ (c_id,c)) msg.
-  Proof.
-    intros.
-    unfold findKeysCrypto.
-    destruct msg; eauto.
-    destruct (c_id ==n c_id0); subst; clean_map_lookups; eauto.
-    simpl in *.
-    specialize (H0 _ eq_refl); contradiction.
-  Qed.
-  
-  Lemma merge_findKeysCrypto_addnl_cipher :
-    forall {t} (msg : crypto t) cs c_id c ks,
-      ~ In c_id cs
-      -> (forall cid, msg_cipher_id msg = Some cid -> cs $? cid <> None)
-      -> ks $k++ findKeysCrypto cs msg = ks $k++ findKeysCrypto (cs $+ (c_id,c)) msg.
-  Proof.
-    intros.
-    erewrite findKeysCrypto_addnl_cipher; trivial.
-  Qed.
-
-  Lemma msg_signed_addressed_addnl_cipher :
-    forall {t} (msg : crypto t) cs c_id c honestk suid,
-      ~ In c_id cs
-      -> (forall cid, msg_cipher_id msg = Some cid -> cs $? cid <> None)
-      -> msg_signed_addressed honestk cs suid msg =
-        msg_signed_addressed honestk (cs $+ (c_id,c)) suid msg.
-  Proof.
-    intros.
-    match goal with
-    | [ |- msg_signed_addressed ?honk ?cs ?suid ?msg = _ ] =>
-      case_eq (msg_signed_addressed honk cs suid msg)
-    end; intros; symmetry; eauto using msg_signed_addressed_nochange_addnl_cipher.
-  Qed.
-
-  Lemma msg_signed_addressed_nochange_addnl_honest_key :
-    forall {t} (msg : crypto t) (gks : keys) honestk cs suid k_id tf,
-      ~ In k_id honestk
-      -> gks $? k_id = None
-      -> (forall k, msg_signing_key cs msg = Some k ->
-              gks $? k <> None /\
-              (honest_key honestk k ->
-               message_no_adv_private honestk cs msg /\ msgCiphersSignedOk honestk cs msg))
-      -> msg_signed_addressed honestk cs suid msg = tf
-      -> msg_signed_addressed (honestk $+ (k_id,true)) cs suid msg = tf.
-  Proof.
-    destruct tf; eauto using msg_signed_addressed_addnl_honest_key; intros.
-    unfold msg_signed_addressed in *; intros.
-    rewrite andb_false_iff in *; split_ors; eauto.
-    left.
-    unfold msg_honestly_signed in *.
-    destruct (msg_signing_key cs msg); eauto.
-    unfold honest_keyb in *.
-    destruct (k_id ==n k); subst; clean_map_lookups; eauto.
-    specialize (H1 _ eq_refl); split_ands; contradiction.
-  Qed.
-
-  Lemma honestk_merge_new_msgs_keys_same :
-    forall honestk cs  {t} (msg : crypto t),
-      message_no_adv_private honestk cs msg
-      -> (honestk $k++ findKeysCrypto cs msg) = honestk.
-  Proof.
-    intros.
-    apply map_eq_Equal; unfold Equal; intros.
-    solve_perm_merges; eauto;
-      specialize (H _ _ Heq0); clean_map_lookups; eauto.
-  Qed.
-
-  Lemma honestk_merge_new_msgs_keys_dec_same :
-    forall honestk {t} (msg : message t),
-      (forall k_id kp, findKeysMessage msg $? k_id = Some kp -> honestk $? k_id = Some true)
-      -> (honestk $k++ findKeysMessage msg) = honestk.
-  Proof.
-    intros.
-    apply map_eq_Equal; unfold Equal; intros.
-    solve_perm_merges; eauto;
-      specialize (H _ _ Heq0); clean_map_lookups; eauto.
-  Qed.
-
-  (* need to know that msg, if cipher, is in cs *)
-  Lemma updateTrackedNonce_addnl_cipher :
-    forall suid nons cs {t} (msg : crypto t) c_id c,
-      ~ In c_id cs
-      -> (forall cid, msg_cipher_id msg = Some cid -> cs $? cid <> None)
-      -> updateTrackedNonce suid nons cs msg =
-        updateTrackedNonce suid nons (cs $+ (c_id, c)) msg.
-  Proof.
-    intros.
-    unfold updateTrackedNonce.
-    destruct msg; eauto.
-    destruct (c_id ==n c_id0); subst; clean_map_lookups; eauto.
-    specialize (H0 _ eq_refl); contradiction.
-  Qed.
-
-  Lemma msg_not_accepted_pattern_addnl_cipher :
-    forall {t} (msg : crypto t) cs suid froms pat c_id c,
-      ~ In c_id cs
-      -> (forall cid, msg_cipher_id msg = Some cid -> cs $? cid <> None)
-      -> ~ msg_accepted_by_pattern cs suid froms pat msg
-      -> ~ msg_accepted_by_pattern (cs $+ (c_id, c)) suid froms pat msg.
-  Proof.
-    intros.
-    unfold not.
-    destruct pat; intros; eauto;
-      repeat
-        match goal with
-        | [ H : msg_accepted_by_pattern _ _ _ _ _ |- _ ] => invert H
-        | [ H : _ $+ (?cid1,_) $? ?cid2 = _ |- _ ] => destruct (cid1 ==n cid2); subst; clean_map_lookups
-        | [ H : ?cs $? ?cid = None,
-                H1 : (forall c_id, _ = Some c_id -> ?cs $? c_id <> None) |- _ ] => simpl in H1; specialize (H1 _ eq_refl); contradiction
-        | [ H : ~ msg_accepted_by_pattern ?cs ?to ?froms ?pat ?m |- _ ] =>
-          assert (msg_accepted_by_pattern cs to froms pat m) by (econstructor; eauto); contradiction
-        end.
-  Qed.
-
-  Lemma msg_accepted_pattern_addnl_cipher :
-    forall {t} (msg : crypto t) cs suid froms pat c_id c,
-      ~ In c_id cs
-      -> msg_accepted_by_pattern cs suid froms pat msg
-      -> msg_accepted_by_pattern (cs $+ (c_id, c)) suid froms pat msg.
-  Proof.
-    intros * NOTIN H; invert H; eauto.
-  Qed.
-
-
-  Lemma msg_accepted_pattern_addnl_cipher_inv :
-    forall {t} (msg : crypto t) cs suid froms pat c_id c,
-      ~ In c_id cs
-      -> (forall cid, msg_cipher_id msg = Some cid -> cs $? cid <> None)
-      -> msg_accepted_by_pattern (cs $+ (c_id, c)) suid froms pat msg
-      -> msg_accepted_by_pattern cs suid froms pat msg.
-  Proof.
-    intros * NOTIN INCS H; invert H; eauto;
-      destruct (c_id ==n c_id0); subst;
-        clean_map_lookups; eauto;
-          simpl in INCS; specialize (INCS _ eq_refl);
-            contradiction.
-  Qed.
-
-  Lemma findKeysCrypto_addnl_cipher' :
-    forall cs cid1 c cid2 t,
-      cid1 <> cid2
-      -> @findKeysCrypto t (cs $+ (cid1, c)) (SignedCiphertext cid2) =
-        @findKeysCrypto t cs (SignedCiphertext cid2).
-  Proof.
-    intros.
-    unfold findKeysCrypto in *; clean_map_lookups; eauto.
-  Qed.
-
-  Lemma updateTrackedNonce_addnl_cipher' :
-    forall cs cid1 c cid2 t nons suid,
-      cid1 <> cid2
-      -> @updateTrackedNonce t suid nons cs (SignedCiphertext cid2) =
-        @updateTrackedNonce t suid nons (cs $+ (cid1, c)) (SignedCiphertext cid2).
-  Proof.
-    intros.
-    unfold updateTrackedNonce; clean_map_lookups; eauto.
-  Qed.
-
-  Hint Resolve
-       findKeysCrypto_addnl_cipher
-       merge_findKeysCrypto_addnl_cipher
-       updateTrackedNonce_addnl_cipher
-       updateTrackedNonce_addnl_cipher'
-       msg_signed_addressed_addnl_cipher
-       msg_signed_addressed_nochange_addnl_honest_key
-       msg_accepted_pattern_addnl_cipher
-       msg_accepted_pattern_addnl_cipher_inv
-       msg_not_accepted_pattern_addnl_cipher
-       : core.
 
   Import SimulationAutomation.
   Import AdversarySafety.Automation.
@@ -1194,197 +1022,6 @@ Section RealWorldLemmas.
                                                    cur_nonce := cur_n; |}
       -> step_universeC U lbl U'. 
 
-  Lemma silent_step_nochange_other_user' :
-    forall {A B C} suid lbl bd bd',
-      step_user lbl suid bd bd'
-      -> forall cs cs' (usrs usrs': honest_users A) (adv adv' : user_data B) gks gks'
-          (cmd cmd' : user_cmd C) ks ks' qmsgs qmsgs' mycs mycs'
-          froms froms' sents sents' cur_n cur_n',
-        bd = (usrs, adv, cs, gks, ks, qmsgs, mycs, froms, sents, cur_n, cmd)
-        -> bd' = (usrs', adv', cs', gks', ks', qmsgs', mycs', froms', sents', cur_n', cmd')
-        -> lbl = Silent
-        -> forall cmdc cmdc' u_id1 u_id2 ud2 usrs'',
-            suid = Some u_id1
-            -> u_id1 <> u_id2
-            -> usrs $? u_id1 = Some {| key_heap := ks;
-                                      protocol := cmdc;
-                                      msg_heap := qmsgs;
-                                      c_heap   := mycs;
-                                      from_nons := froms;
-                                      sent_nons := sents;
-                                      cur_nonce := cur_n |}
-            -> usrs $? u_id2 = Some ud2
-            -> usrs'' = usrs' $+ (u_id1, {| key_heap := ks';
-                                           protocol := cmdc';
-                                           msg_heap := qmsgs';
-                                           c_heap   := mycs';
-                                           from_nons := froms';
-                                           sent_nons := sents';
-                                           cur_nonce := cur_n' |})
-            -> usrs'' $? u_id2 = Some ud2.
-  Proof.
-    induction 1; inversion 1; inversion 1;
-      intros; subst;
-        try discriminate;
-        try solve [ clean_map_lookups; trivial ].
-    specialize (IHstep_user _ _ _ _ _ _ _ _ _ _ _
-                            _ _ _ _ _ _ _ _ _ _ _
-                            eq_refl eq_refl eq_refl).
-    specialize (IHstep_user cmdc cmdc').
-    specialize (IHstep_user _ _ _ _ eq_refl H26 H27 H28 eq_refl).
-    clean_map_lookups; eauto.
-  Qed.
-
-  Lemma silent_step_nochange_other_user :
-    forall {A B} suid lbl bd bd',
-      step_user lbl suid bd bd'
-      -> forall cs cs' (usrs usrs': honest_users A) (adv adv' : user_data B) gks gks'
-          cmd cmd' ks ks' qmsgs qmsgs' mycs mycs'
-          froms froms' sents sents' cur_n cur_n',
-        bd = (usrs, adv, cs, gks, ks, qmsgs, mycs, froms, sents, cur_n, cmd)
-        -> bd' = (usrs', adv', cs', gks', ks', qmsgs', mycs', froms', sents', cur_n', cmd')
-        -> lbl = Silent
-        -> forall u_id1 u_id2 ud2 usrs'',
-            suid = Some u_id1
-            -> u_id1 <> u_id2
-            -> usrs $? u_id1 = Some {| key_heap := ks;
-                                      protocol := cmd;
-                                      msg_heap := qmsgs;
-                                      c_heap   := mycs;
-                                      from_nons := froms;
-                                      sent_nons := sents;
-                                      cur_nonce := cur_n |}
-            -> usrs $? u_id2 = Some ud2
-            -> usrs'' = usrs' $+ (u_id1, {| key_heap := ks';
-                                           protocol := cmd';
-                                           msg_heap := qmsgs';
-                                           c_heap   := mycs';
-                                           from_nons := froms';
-                                           sent_nons := sents';
-                                           cur_nonce := cur_n' |})
-            -> usrs'' $? u_id2 = Some ud2.
-  Proof.
-    intros; subst; eapply silent_step_nochange_other_user'; eauto.
-  Qed.
-
-  Lemma step_limited_change_other_user' :
-    forall {A B C} suid lbl bd bd',
-      step_user lbl suid bd bd'
-      -> forall cs cs' (usrs usrs': honest_users A) (adv adv' : user_data B) gks gks'
-          (cmd cmd' : user_cmd C) ks ks' qmsgs qmsgs' mycs mycs'
-          froms froms' sents sents' cur_n cur_n',
-        bd = (usrs, adv, cs, gks, ks, qmsgs, mycs, froms, sents, cur_n, cmd)
-        -> bd' = (usrs', adv', cs', gks', ks', qmsgs', mycs', froms', sents', cur_n', cmd')
-        -> forall cmdc cmdc' u_id1 u_id2 usrs'' ks2 cmdc2 qmsgs2 mycs2 froms2 sents2 cur_n2,
-            suid = Some u_id1
-            -> u_id1 <> u_id2
-            -> usrs $? u_id1 = Some {| key_heap := ks;
-                                      protocol := cmdc;
-                                      msg_heap := qmsgs;
-                                      c_heap   := mycs;
-                                      from_nons := froms;
-                                      sent_nons := sents;
-                                      cur_nonce := cur_n |}
-            -> usrs $? u_id2 = Some {| key_heap := ks2;
-                                      protocol := cmdc2;
-                                      msg_heap := qmsgs2;
-                                      c_heap   := mycs2;
-                                      from_nons := froms2;
-                                      sent_nons := sents2;
-                                      cur_nonce := cur_n2 |}
-            -> usrs'' = usrs' $+ (u_id1, {| key_heap := ks';
-                                           protocol := cmdc';
-                                           msg_heap := qmsgs';
-                                           c_heap   := mycs';
-                                           from_nons := froms';
-                                           sent_nons := sents';
-                                           cur_nonce := cur_n' |})
-            -> (forall cid c, cs $? cid = Some c -> cs' $? cid = Some c)
-            /\ ( usrs'' $? u_id2 = Some {| key_heap := ks2;
-                                          protocol := cmdc2;
-                                          msg_heap := qmsgs2;
-                                          c_heap   := mycs2;
-                                          from_nons := froms2;
-                                          sent_nons := sents2;
-                                          cur_nonce := cur_n2 |}
-              \/ exists m,
-                usrs'' $? u_id2 = Some {| key_heap := ks2;
-                                          protocol := cmdc2;
-                                          msg_heap := qmsgs2 ++ [m];
-                                          c_heap   := mycs2;
-                                          from_nons := froms2;
-                                          sent_nons := sents2;
-                                          cur_nonce := cur_n2 |} )
-  .
-  Proof.
-    induction 1; inversion 1; inversion 1;
-      intros; subst;
-        try solve [ split; [intros | left; clean_map_lookups; trivial]; eauto ].
-    
-    - specialize (IHstep_user _ _ _ _ _ _ _ _ _ _ _
-                              _ _ _ _ _ _ _ _ _ _ _
-                              eq_refl eq_refl).
-      specialize (IHstep_user cmdc cmdc').
-      specialize (IHstep_user _ _ _ _ _ _ _ _ _ _ eq_refl H25 H26 H27 eq_refl).
-      split_ors; eauto.
-
-    - split; [ | clean_context; clean_map_lookups]; eauto.
-      destruct (rec_u_id ==n u_id2); subst; eauto.
-  Qed.
-
-  Lemma step_limited_change_other_user :
-    forall {A B} suid lbl bd bd',
-      step_user lbl suid bd bd'
-      -> forall cs cs' (usrs usrs': honest_users A) (adv adv' : user_data B) gks gks'
-          cmd cmd' ks ks' qmsgs qmsgs' mycs mycs'
-          froms froms' sents sents' cur_n cur_n',
-
-        bd = (usrs, adv, cs, gks, ks, qmsgs, mycs, froms, sents, cur_n, cmd)
-        -> bd' = (usrs', adv', cs', gks', ks', qmsgs', mycs', froms', sents', cur_n', cmd')
-        -> forall u_id1 u_id2 usrs'' ks2 qmsgs2 mycs2 froms2 sents2 cur_n2 cmd2,
-            suid = Some u_id1
-            -> u_id1 <> u_id2
-            -> usrs $? u_id1 = Some {| key_heap := ks;
-                                      protocol := cmd;
-                                      msg_heap := qmsgs;
-                                      c_heap   := mycs;
-                                      from_nons := froms;
-                                      sent_nons := sents;
-                                      cur_nonce := cur_n |}
-            -> usrs $? u_id2 = Some {| key_heap := ks2;
-                                      protocol := cmd2;
-                                      msg_heap := qmsgs2;
-                                      c_heap   := mycs2;
-                                      from_nons := froms2;
-                                      sent_nons := sents2;
-                                      cur_nonce := cur_n2 |}
-            -> usrs'' = usrs' $+ (u_id1, {| key_heap := ks';
-                                           protocol := cmd';
-                                           msg_heap := qmsgs';
-                                           c_heap   := mycs';
-                                           from_nons := froms';
-                                           sent_nons := sents';
-                                           cur_nonce := cur_n' |})
-            -> (forall cid c, cs $? cid = Some c -> cs' $? cid = Some c)
-            /\ ( usrs'' $? u_id2 = Some {| key_heap := ks2;
-                                         protocol := cmd2;
-                                         msg_heap := qmsgs2;
-                                         c_heap   := mycs2;
-                                         from_nons := froms2;
-                                         sent_nons := sents2;
-                                         cur_nonce := cur_n2 |}
-              \/ exists m,
-                usrs'' $? u_id2 = Some {| key_heap := ks2;
-                                          protocol := cmd2;
-                                          msg_heap := qmsgs2 ++ [m];
-                                          c_heap   := mycs2;
-                                          from_nons := froms2;
-                                          sent_nons := sents2;
-                                          cur_nonce := cur_n2 |})
-  .
-  Proof.
-    intros; subst; eapply step_limited_change_other_user'; eauto.
-  Qed.
 
 End RealWorldLemmas.
 
@@ -1578,15 +1215,6 @@ Section AuxDefinitions.
       eexists; split; eauto.
       
   Qed.
-
-  (* (* This encoding sucks *) *)
-  (* Inductive boundRunningTimeUniv {A} : list (user_id * user_data A) -> nat -> Prop := *)
-  (* | BrtEmpty : boundRunningTimeUniv [] 0 *)
-  (* | BrtRecur : forall uid u us n n', *)
-  (*     boundRunningTime u.(protocol) n *)
-  (*     -> boundRunningTimeUniv us n' *)
-  (*     -> boundRunningTimeUniv ((uid,u) :: us) (n + n') *)
-  (* . *)
 
   Inductive boundRunningTimeUniv {A} : honest_users A -> nat -> Prop :=
   | BrtEmpty : boundRunningTimeUniv $0 0
@@ -1988,19 +1616,52 @@ Lemma alignment_violations_translate :
 Proof.
 Admitted.
 
-(* Theorem step_stepC : *)
-(*   forall {t__hon t__adv} (ru0 : RealWorld.universe t__hon t__adv) (iu0 : IdealWorld.universe t__hon), *)
-(*   (* summarizeThreads c cs *) *)
-(*     (* -> boundRunningTime c n *) *)
+Theorem step_stepC :
+  forall {t__hon t__adv} (ru0 : RealWorld.universe t__hon t__adv) (iu0 : IdealWorld.universe t__hon) b,
+    (* -> boundRunningTime c n *)
+    syntactically_safe_U ru0
+    -> lameAdv b ru0.(adversary)
+    -> invariantFor (TrC ru0 iu0) (fun st => no_resends_U (fst st) /\ labels_align st)
+    -> invariantFor (S ru0 iu0) (fun st => safety st /\ labels_align st)
+.
+Proof.
+  intros * SYN_SAFE LAME INV.
 
-(*     (* typechecked protocol + typechecker sound *) *)
-(*     invariantFor (TrC ru0 iu0) (fun st => msg_not_resent st /\ labels_align st) *)
-(*     -> invariantFor (S ru0 iu0) (fun st => safety st /\ labels_align st) *)
-(* . *)
-(* Proof. *)
-(*   intros * INV. *)
-(*   unfold invariantFor in *; intros * INIT. *)
-(*   simpl in *. *)
-(*   specialize (INV _ INIT); intros. *)
+  apply NNPP; unfold not; intros INV'.
+  unfold invariantFor in INV'.
+  apply not_all_ex_not in INV'; split_ex.
+  apply imply_to_and in H; split_ex.
+  apply not_all_ex_not in H0; split_ex.
+  apply imply_to_and in H0; split_ex.
+  simpl in H; split_ors; try contradiction.
+  destruct x0 as [?ru ?iu].
 
-(* Admitted. *)
+  apply not_and_or in H1; split_ors.
+  unfold safety in H1.
+
+
+  (* subst. *)
+  (* simplify. *)
+  (* cases (notAboutToFail c); propositional. *)
+  (* assert (exists n', boundRunningTime c n' /\ n' <= n) by eauto using boundRunningTime_steps. *)
+  (* first_order. *)
+  (* eapply complete_trace in H2; eauto. *)
+  (* first_order. *)
+  (* specialize (trc_trans H4 H2); simplify. *)
+  (* assert (notAboutToFail x2 = false) by eauto using notAboutToFail_steps. *)
+  (* unfold invariantFor in H1; simplify. *)
+  (* apply steps_stepsi in H7; first_order. *)
+  (* eapply translate_trace in H7; eauto. *)
+  (* first_order. *)
+  (* apply H1 in H7; auto. *)
+  (* equality. *)
+
+
+
+
+  
+  (* unfold invariantFor in *; intros * INIT. *)
+  (* simpl in *. *)
+  (* specialize (INV _ INIT); intros. *)
+
+Admitted.
